examples/Gen_sym/Gen_sym.mli
@@ -3,20 +3,20 @@
 type name
 (*@ model : name *)
 
-type t
+type gen
 (*@ mutable model : name Set.t *)
 
-val create : unit -> t
+val create : unit -> gen
 (*@ let g = create () in
       ensures g = Set.empty *)
 
-val next : t -> name
-(*@ let n = next g in
-      ensures Set.mem n g
+val next : gen -> name
+(*@ modifies g
+    let n = next g in
       ensures not (Set.mem n (old g))
-      ensures Set.subset (old g) g *)
+      ensures g = Set.add n (old g) *)
 
-val reset : t -> unit
+val reset : gen -> unit
 (*@ modifies g
     let () = reset g in
       ensures g = Set.empty *)
