examples/Gen_sym/Gen_sym_proof.v
@@ -4,3 +4,95 @@ From CFML Require Import Stdlib.
 From TLC Require Import LibListZ.
 
 From EXAMPLES Require Import Gen_sym_ml.
+
+Require Import Gospelstdlib_verified.
+
+Import Gospelstdlib.
+
+Definition __ocaml_name := Z.
+Definition name := Z.
+
+Instance __Inhab_name : Inhab __ocaml_name := Inhab_int.
+
+Instance __Enc_name : Enc __ocaml_name := Enc_int.
+
+Definition Name (y : name) (x : val) : hprop := \[x = y].
+
+Definition Gen (s : _Set.t name) (l : loc) : hprop :=
+  \exists n,
+    l ~~> n \*
+      \[n >= 0] \*
+      \[forall m, 0 < m <= n -> _Set.mem m s] \*
+      \[forall m, m <= 0 \/ m > n -> ~ (_Set.mem m s)].
+
+(* Definition Gen' s (v : val) := exists l, v = VLoc l /\ Gen s l. *)
+
+Definition _create : val := create.
+
+Lemma initial_spec : initial = 0.
+Proof. xcf. Qed.
+
+Lemma _create_spec :
+  SPEC(_create tt)
+  PRE\[]
+  POST(fun _prog_g : loc => (_prog_g ~> Gen _Set.empty)).
+Proof using.
+  unfold _create.
+  xcf. xapp*.
+  xunfold Gen. xsimpl; intros.
+  1, 2: rewrite initial_spec in *; math.
+  apply _Set.empty_mem.
+Qed.
+
+Definition _next : val := next.
+
+Definition _next_spec :
+  forall _prog_g : loc,
+  forall g : _Set.t name,
+  SPEC(_next _prog_g)
+  PRE((_prog_g ~> Gen g))
+  POST(
+    fun _prog_n : name =>
+    \exists n : name,
+    ((_prog_g ~> Gen (_Set.add n g)) \* (_prog_n ~> Name n))
+  ).
+Proof using.
+  unfold _next.
+  xcf. xunfold Gen. xpull. intros x H1 H2 H3.
+  xapp. xapp. xapp. xif. intros; math.
+  intros H4. xval. xapp. xsimpl.
+  Unshelve. 5: apply (x + 1).
+
+  - math.
+  - intros m H5.
+    assert (A : m = x + 1 \/ m <> x + 1).
+    { apply classic. }
+    destruct A.
+    + subst. apply _Set.add_mem.
+    + apply _Set.add_mem_neq.
+      auto. apply H2. math.
+  - intros m H5. destruct H5;
+    rewrite <- _Set.add_mem_neq.
+    + auto.
+    + math.
+    + apply H3. right. math.
+    + math.
+  - xunfold Name. xsimpl. auto.
+Qed.
+
+Definition _reset : val := reset.
+
+Lemma _reset_spec :
+  forall _prog_g : loc,
+  forall g : _Set.t name,
+  SPEC(_reset _prog_g)
+  PRE((_prog_g ~> Gen g))
+  POST(fun _ : unit => (_prog_g ~> Gen _Set.empty)).
+Proof.
+  unfold _reset. xcf.
+  xunfold Gen. xpull. intros x H1 H2 H3.
+  xapp. xsimpl.
+  2, 3: intros m H4.
+  1, 2: rewrite initial_spec in *; math.
+  apply _Set.empty_mem.
+Qed.
